Working for OVN

coq_ssprove/src/Hacspec_Lib.v
@@ -49,8 +49,6 @@ Import choice.Choice.Exports.
 (*   bind_both_ z (fun z' => *)
 (*   ret_both (f x' y' z')))). *)
 
-
-
 Equations int_add {L1 L2 (* L3 *) : {fset Location}} {I1 I2 (* I3 *) : Interface} {WS}
            (x : both L1 I1 (int WS)) (y : both L2 I2 (int WS))
            (* `{H_loc_incl_x : is_true (fsubset L1 L3)} `{H_opsig_incl_x : is_true (fsubset I1 I3)} *)
@@ -248,14 +246,22 @@ Section Loops.
   Solve All Obligations with (intros ; (fset_equality || solve_in_fset)).
   Fail Next Obligation.
 
-  Program Definition foldi_both_
+  (* Obligation Tactic := (intros ; (fset_equality || solve_in_fset)). *)
+  Equations foldi_both_
            {acc : choice_type}
            (fuel : nat)
            {L1 L2 I1 I2}
            (i : both L2 I2 uint_size)
-           (f: forall {L I} `{is_true (fsubset L1 L)} `{is_true (fsubset I1 I)}, both L2 I2 (uint_size) -> both L I acc -> both (L :|: L2) (I :|: I2) (acc))
-           (cur : both L1 I1 acc) : both (L1 :|: L2) (I1 :|: I2) (acc) :=
-      foldi_ (L := L1 :|: L2) fuel i (@f (L1 :|: L2) (I1 :|: I2) (fsubsetUl _ _) (fsubsetUl _ _)) (lift_both cur (fsubset_loc := _) (fsubset_opsig := _)) (fsubset_loc := _) (fsubset_opsig := _).
+           {L I}
+           `{is_true (fsubset L1 L)} `{is_true (fsubset I1 I)}
+           `{is_true (fsubset L2 L)} `{is_true (fsubset I2 I)}
+           (f: both L2 I2 (uint_size) -> both L I acc -> both L I (acc))
+           (cur : both L1 I1 acc) : both L I (acc) :=
+    foldi_both_ fuel i f cur :=
+      match fuel with
+      | 0 => lift_both cur
+      | S n' => solve_lift foldi_both_ n' (int_add i (ret_both one)) (fun x y => solve_lift f (solve_lift x) y) (f i (solve_lift cur))
+      end.
   Solve All Obligations with (intros ; (fset_equality || solve_in_fset)).
   Fail Next Obligation.
 
@@ -264,8 +270,12 @@ Section Loops.
              {L1 L2 L3 I1 I2 I3}
              (lo: both L2 I2 uint_size)
              (hi: both L3 I3 uint_size) (* {lo <= hi} *)
-             (f: forall {L I}  `{is_true (fsubset L1 L)} `{is_true (fsubset I1 I)}, both (L2 :|: L3) (I2 :|: I3) (uint_size) -> both L I acc -> both (L :|: (L2 :|: L3)) (I :|: (I2 :|: I3)) (acc)) (* {i < hi} *)
-             (init: both L1 I1 acc) : both (L1 :|: (L2 :|: L3)) (I1 :|: (I2 :|: I3)) (acc) :=
+             {L I}
+           `{is_true (fsubset L1 L)} `{is_true (fsubset I1 I)}
+           `{is_true (fsubset L2 L)} `{is_true (fsubset I2 I)}
+           `{is_true (fsubset L3 L)} `{is_true (fsubset I3 I)}
+           (f: both (L2 :|: L3) (I2 :|: I3) (uint_size) -> both L I acc -> both L I (acc)) (* {i < hi} *)
+             (init: both L1 I1 acc) : both L I (acc) :=
     foldi lo hi f init :=
       bind_both lo (fun lo =>
       bind_both hi (fun hi =>
@@ -1104,13 +1114,14 @@ Infix "seq_xor" := seq_xor_ (at level 33) : hacspec_scope.
     | y :: ys =>
         bind_both x (fun temp_x =>
         bind_both (array_from_list_helper y ys k) (fun temp_y =>
-        solve_lift (ret_both (setm (temp_y : nseq_ A (S k)) (Ordinal (ssrbool.introT ssrnat.ltP (lt_succ_diag_r_sub k (length (y :: ys))))) temp_x : nseq_ A (S k)))) (fsubset_loc := _)  (fsubset_opsig := _)) (fsubset_loc := _)  (fsubset_opsig := _)
+        lift_both (fsubset_loc := _) (fsubset_opsig := _) (ret_both (setm (temp_y : nseq_ A (S k)) (Ordinal (ssrbool.introT ssrnat.ltP (lt_succ_diag_r_sub k (length (y :: ys))))) temp_x : nseq_ A (S k)))) (fsubset_loc := _)  (fsubset_opsig := _)) (fsubset_loc := _)  (fsubset_opsig := _)
     end.
-  Solve All Obligations with (intros ; time (fset_equality || solve_in_fset)).
+  Solve All Obligations with (intros ; (* time *) (fset_equality || solve_in_fset)).
   Fail Next Obligation.
 
-  Program Definition array_from_list {A: choice_type} {L I} (l: list (both L I A))
+  Equations array_from_list {A: choice_type} {L I} (l: list (both L I A))
     : both L I (nseq_ A (length l)) :=
+    array_from_list l :=
     match l as k return both L I (nseq_ A (length k)) with
       [] => solve_lift (ret_both (tt : nseq_ A 0))
     | (x :: xs) => array_from_list_helper x xs (length xs)
@@ -1459,8 +1470,71 @@ Definition result_unwrap_safe {a b} (x : result b a) `{match x with inl _ => Tru
 
 Module choice_typeMonad.
 
-  Class BindCode (M : choice_type -> choice_type) `{mnd : @choice_typeMonad.CEMonad M}  :=
-    { bind_code [L : {fset Location}] {I} {A B : choice_type} (x : code L I (M A)) (f : A -> code L I (M B)) : code L I (M B) }.
+  Class BindCode :=
+    {
+      mnd :> choice_typeMonad.CEMonad ;
+      (* bind_code {L : {fset Location}} {I} {A B : choice_type} (x : code L I (choice_typeMonad.M A)) (f : A -> code L I (choice_typeMonad.M B)) : code L I (choice_typeMonad.M B) ; *)
+      monad_bind_both {L0 L1 : {fset Location}} {I0 I1} {A B : choice_type} (x : both L0 I0 (choice_typeMonad.M (CEMonad := mnd) A)) (f : both L0 I0 A -> both L1 I1 (choice_typeMonad.M (CEMonad := mnd) B)) `{fsubset_loc : is_true (fsubset L0 L1)} `{fsubset_opsig : is_true (fsubset I0 I1)} : both L1 I1 (choice_typeMonad.M (CEMonad := mnd) B) ;
+    }.
+
+
+  (* Definition both_to_code {L I A} : both L I A -> code L I A := *)
+  (*   fun x => {| prog := is_state x ; prog_valid := is_valid_code (both_prog_valid x) |}. *)
+
+  (* Program Definition monad_bind_both `{BindCode} [L : {fset Location}] {I} {A B : choice_type} (x : both L I (choice_typeMonad.M A)) (f : both L I A -> both L I (choice_typeMonad.M B)) : both L I (choice_typeMonad.M B) := *)
+  (*   {| *)
+  (*     both_prog := *)
+  (*     {| *)
+  (*       is_pure := @choice_typeMonad.bind mnd A B (is_pure x) (fun x => is_pure (f (solve_lift (ret_both x)))) ; *)
+  (*       is_state := prog (bind_code (both_to_code x) (fun a => both_to_code (f (solve_lift ret_both a)))) ; *)
+  (*     |} ; *)
+  (*     both_prog_valid := {| *)
+  (*                         is_valid_code := prog_valid _ ; *)
+  (*                         is_valid_both := _ ; *)
+  (*                       |}; *)
+  (*   |}. *)
+  (* Solve All Obligations with (intros ; (fset_equality || solve_in_fset)). *)
+  (* Next Obligation. *)
+  (*   intros. *)
+  (*   destruct x. *)
+  (*   simpl. *)
+  (*   unfold both_to_code. *)
+  (*   simpl. *)
+
+  (*   unfold choice_typeMonad.bind. *)
+  (*   destruct is_valid_both. *)
+  (*   epose choice_typeMonad.monad_law1. *)
+  (*   epose choice_typeMonad.monad_law2. *)
+  (*   epose choice_typeMonad.monad_law3. *)
+
+  (*   simpl. *)
+
+
+  (*   simpl. *)
+
+
+  (*   rewrite choice_typeMonad.monad_law1. *)
+
+  (*   rewrite bind_ret. *)
+
+  (*   apply both_valid_ret. *)
+  (*   simpl. *)
+  (*   apply  *)
+  (*   eapply bind_both. *)
+  (*   apply x. *)
+  (*   intros. *)
+  (*   refine (f _). *)
+  (*   epose (choice_typeMonad.bind X (fun a => f _)). *)
+  (*   refine (solve_lift ret_both (choice_typeMonad.bind X (fun a' => f))). *)
+
+  (*   intros. *)
+  (*   refine (). *)
+
+  (*   epose (bind_code (is_state x) f). *)
+  (*   eapply s. *)
+  (*   apply x. *)
+  (*   apply f. *)
+  (*   apply x. *)
 
   (* Class BindBoth (M : choice_type -> choice_type) `{mnd : @choice_typeMonad.CEMonad M} `{H_bind_code : @BindCode M mnd} := *)
   (*    { *)
@@ -1490,22 +1564,16 @@ Module choice_typeMonad.
   (*   apply code_ext. apply H1. *)
   (* Qed. *)
 
-  #[global] Program Instance result_bind_code C : BindCode (result C) :=
-    {| bind_code L I A B x f :=
-      {code t_x ← x ;;
-       match t_x with
-       | inl s => f s
-       | inr s => ret (Err s)
-       end} |}.
-  Next Obligation.
-    intros.
-    apply valid_bind.
-    apply prog_valid.
-    intros; cbn.
-    destruct x0.
-    - apply prog_valid.
-    - apply valid_ret.
-  Qed.
+  #[global] Program Instance result_bind_code C : BindCode :=
+    {|
+      mnd := (@choice_typeMonad.result_monad C) ;
+      monad_bind_both _ _ _ _ _ _ x f _ _ := bind_both x (fun x => match x with
+                                                        | inl s => f (solve_lift ret_both s)
+                                                        | inr s => solve_lift ret_both (Err s)
+                                                        end)
+    |}.
+  Solve All Obligations with (intros ; (fset_equality || solve_in_fset)).
+  Fail Next Obligation.
 
   (* #[global] Program Instance result_bind_both C : BindBoth (result C). *)
   (* Next Obligation. *)
@@ -1521,22 +1589,16 @@ Module choice_typeMonad.
   (*   - now apply r_ret. *)
   (* Qed. *)
 
-  #[global] Program Instance option_bind_code : BindCode (option) :=
-    {| bind_code L I A B x f :=
-      {code t_x ← x ;;
+  #[global] Program Instance option_bind_code : BindCode :=
+    {| mnd := choice_typeMonad.option_monad;
+      monad_bind_both _ _ _ _ A B x f _ _ :=
+      bind_both x (fun t_x =>
        match t_x with
-       | Some s => f s
-       | None => ret ((@None B : option B))
-       end} |}.
-  Next Obligation.
-    intros.
-    apply valid_bind.
-    apply prog_valid.
-    intros; cbn.
-    destruct x0.
-    - apply prog_valid.
-    - apply valid_ret.
-  Qed.
+       | Some s => f (solve_lift ret_both s)
+       | None => solve_lift ret_both (@None B : option B)
+       end) |}.
+  Solve All Obligations with (intros ; (fset_equality || solve_in_fset)).
+  Fail Next Obligation.
 
   (* #[global] Program Instance option_bind_both : BindBoth (option). *)
   (* Next Obligation. *)
@@ -1553,6 +1615,16 @@ Module choice_typeMonad.
   (* Qed. *)
 
 End choice_typeMonad.
+
+(* Notation "'bind_exception' t' x ':=' y 'in' z" := ( *)
+(*   choice_typeMonad.bind_code (BindCode := t) *)
+(*                              (A := _) (B := _) (L := _) *)
+(*                              (y) (fun x => z)) (at level 99). *)
+(* Notation Result t := (@choice_typeMonad.result_monad t). *)
+
+(* Definition run (x : Exception A B) : Result A B. *)
+
+(* Definition run (x : result B A). *)
 
 (*** Result *)
 
@@ -1571,17 +1643,17 @@ Definition Err  {L I} {a b : choice_type} : both L I b -> both L I (result b a) 
 (* Notation "'letbnd(' M ')' x ':=' y 'in' f" := (choice_typeMonad.bind_both (BindBoth := M) (lift_scope (H_loc_incl := _) (H_opsig_incl := _) y) (fun x => f)) (at level 100, x pattern, right associativity). *)
 (* Notation "'letbnd(' M ')' ' x ':=' y 'in' f" := (choice_typeMonad.bind_both (BindBoth := M) (lift_scope (H_loc_incl := _) (H_opsig_incl := _) y) (fun x => f)) (at level 100, x pattern, right associativity). *)
 
-Program Definition bind_code_mut  {L : {fset Location}} {I} `{H_bind_code : choice_typeMonad.BindCode} {B : choice_type} (x_loc : Location) {A : choice_type} `{H_loc : M A = (x_loc)} `{H_in: is_true (ssrbool.in_mem (x_loc) (ssrbool.mem L))} (x : code L I (x_loc)) (f : A -> code L I (M B)) : code L I (M B) .
-Proof.
-  destruct x_loc as [? n].
-  cbn in *. subst.
-  refine ({code choice_typeMonad.bind_code x (fun temp => {code
-         #put ((M A) ; n) := (choice_typeMonad.ret temp) ;;
-                                f temp}) }).
-Defined.
+(* Program Definition bind_code_mut  {L : {fset Location}} {I} `{H_bind_code : choice_typeMonad.BindCode} {B : choice_type} (x_loc : Location) {A : choice_type} `{H_loc : M A = (x_loc)} `{H_in: is_true (ssrbool.in_mem (x_loc) (ssrbool.mem L))} (x : code L I (x_loc)) (f : A -> code L I (M B)) : code L I (M B) . *)
+(* Proof. *)
+(*   destruct x_loc as [? n]. *)
+(*   cbn in *. subst. *)
+(*   refine ({code choice_typeMonad.bind_code x (fun temp => {code *)
+(*          #put ((M A) ; n) := (choice_typeMonad.ret temp) ;; *)
+(*                                 f temp}) }). *)
+(* Defined. *)
 
-Notation "'bndm(' M ',' A ',' B ',' L ')' x 'loc(' ℓ ')'  '⇠' y 'in' f" := (bind_code_mut (H_bind_code := M) (A := A) (B := B) (L := L) (H_loc := eq_refl) ℓ y (fun x => f)) (at level 100, x pattern, right associativity).
-Notation "'bndm(' M ',' A ',' B ',' L ')' ' x 'loc(' ℓ ')'  '⇠' y 'in' f" := (bind_code_mut (H_bind_code := M) (A := A) (B := B) (L := L) (H_loc := eq_refl) ℓ y (fun x => f)) (at level 100, x pattern, right associativity).
+(* Notation "'bndm(' M ',' A ',' B ',' L ')' x 'loc(' ℓ ')'  '⇠' y 'in' f" := (bind_code_mut (H_bind_code := M) (A := A) (B := B) (L := L) (H_loc := eq_refl) ℓ y (fun x => f)) (at level 100, x pattern, right associativity). *)
+(* Notation "'bndm(' M ',' A ',' B ',' L ')' ' x 'loc(' ℓ ')'  '⇠' y 'in' f" := (bind_code_mut (H_bind_code := M) (A := A) (B := B) (L := L) (H_loc := eq_refl) ℓ y (fun x => f)) (at level 100, x pattern, right associativity). *)
 
 
 (* Definition bind_both_mut  {L : {fset Location}} {I} {A B : choice_type} (x_loc : Location) `{H_in: is_true (ssrbool.in_mem (x_loc) (ssrbool.mem L))} `{H_bind_both : choice_typeMonad.BindBoth} {H_loc : M A = (x_loc)} (x : both L I (x_loc)) (f : A -> both L I (M B)) : both L I (M B). *)
@@ -1612,8 +1684,8 @@ Notation "'bndm(' M ',' A ',' B ',' L ')' ' x 'loc(' ℓ ')'  '⇠' y 'in' f" :=
 (*   easy. *)
 (* Defined. *)
 
-Notation "'bndm(' M ',' A ',' B ',' L ')' x '⇠' y 'in' f" := (choice_typeMonad.bind_code (BindCode := M) (A := A) (B := B) (L := L) y (fun x => f)) (at level 100, x pattern, right associativity).
-Notation "'bndm(' M ',' A ',' B ',' L ')' ' x '⇠' y 'in' f" := (choice_typeMonad.bind_code (BindCode := M) (A := A) (B := B) (L := L) y (fun x => f)) (at level 100, x pattern, right associativity).
+(* Notation "'bndm(' M ',' A ',' B ',' L ')' x '⇠' y 'in' f" := (choice_typeMonad.bind_code (BindCode := M) (A := A) (B := B) (L := L) y (fun x => f)) (at level 100, x pattern, right associativity). *)
+(* Notation "'bndm(' M ',' A ',' B ',' L ')' ' x '⇠' y 'in' f" := (choice_typeMonad.bind_code (BindCode := M) (A := A) (B := B) (L := L) y (fun x => f)) (at level 100, x pattern, right associativity). *)
 
 (* Notation "'letbndm(' M ')' x ':=' y 'in' f" := (choice_typeMonad.bind_both (BindBoth := M) (lift_scope (H_loc_incl := _) (H_opsig_incl := _) y) (fun x => f)) (at level 100, x pattern, right associativity). *)
 (* Notation "'letbndm(' M ')' ' x ':=' y 'in' f" := (choice_typeMonad.bind_both (BindBoth := M) (lift_scope (H_loc_incl := _) (H_opsig_incl := _) y) (fun x => f)) (at level 100, x pattern, right associativity). *)
@@ -2150,15 +2222,15 @@ Proof.
     reflexivity.
 Qed.
 
-Definition andb (x y : 'bool) : both (fset []) ([interface]) 'bool := ret_both (andb x y : 'bool).
+(* Definition andb (x y : 'bool) : both (fset []) ([interface]) 'bool := ret_both (andb x y : 'bool). *)
 
 Infix "&&" := andb : bool_scope.
 
-Definition orb (x y : 'bool) : both (fset []) ([interface]) 'bool := ret_both (orb x y : 'bool).
+(* Definition orb (x y : 'bool) : both (fset []) ([interface]) 'bool := ret_both (orb x y : 'bool). *)
 
 Infix "||" := orb : bool_scope.
 
-Definition negb (x : 'bool) : both (fset []) ([interface]) 'bool := ret_both (negb x : 'bool).
+(* Definition negb (x : 'bool) : both (fset []) ([interface]) 'bool := ret_both (negb x : 'bool). *)
 
 (* Program Definition ret_both  {L : {fset Location}} {I} `{choice_typeMonad.CEMonad} {A : choice_type} (x : A) : both L I (M A) := ret_both (choice_typeMonad.ret x). *)
 
@@ -2528,22 +2600,13 @@ Notation "'ssp' ( 'fun' a => f )" :=
   (((fun (a : both _ _ _) => f)) (* : both _ _ uint_size -> both _ _ _ -> both _ _ _ *)) (at level 100, f at next level, a at next level).
 
 Notation "'ssp' ( 'fun' ' ( a , b ) => f )" :=
-  (((fun (temp : both _ _ (_ × _)) =>
-       letb '(a, b) := (* split_both *) temp in
-       (* let '(a, b) := unsplit_both_all(a, b) in *)
-       f)) (* : both _ _ uint_size -> both _ _ (_ × _) -> both _ _ _ *)) (at level 100, f at next level, a at next level, b at next level).
+  (fun (temp : both _ _ (_ × _)) => lift_n 1 temp (fun '(a, b) => f)) (at level 100, f at next level, a at next level, b at next level).
 
 Notation "'ssp' ( 'fun' ' ( a , b , c ) => f )" :=
-  (((fun (temp : both _ _ (_ × _ × _)) =>
-       letb '(a, b, c) := (* split_both *) temp in
-       (* let '(a, b, c) := unsplit_both_all(a, b, c) in *)
-     f)) (* : both _ _ uint_size -> both _ _ (_ × _ × _) -> both _ _ _ *)) (at level 100, f at next level, a at next level, b at next level, c at next level).
+  (fun (temp : both _ _ (_ × _ × _)) => lift_n 2 temp (fun '(a, b, c) => f)) (at level 100, f at next level, a at next level, b at next level, c at next level).
 
 Notation "'ssp' ( 'fun' ' ( a , b , c , d ) => f )" :=
-  (((fun (temp : both _ _ (_ × _ × _ × _)) =>
-       letb '(a, b, c, d) := (* split_both *) temp in
-       (* let '(a, b, c, d) := unsplit_both_all(a,b,c,d) in *)
-       f)) (* : both _ _ uint_size -> both _ _ (_ × _ × _ × _) -> both _ _ _ *)) (at level 100, f at next level, a at next level, b at next level, c at next level, d at next level).
+  (fun (temp : both _ _ (_ × _ × _ × _)) => lift_n 3 temp (fun '(a, b, c, d) => f)) (at level 100, f at next level, a at next level, b at next level, c at next level, d at next level).
 
 (* eq_fset *)
 (* finmap.finSet *)
@@ -2627,22 +2690,22 @@ Ltac solve_zero :=
 (*   rewrite loc_list_incl_fsubset ; *)
 (*   loc_incl_compute. *)
 
-Check in_fsetU.
 Ltac solve_in_mem :=
   (* match goal with *)
   (* | [ |- context [ ssrbool.in_mem _ (ssrbool.mem _) ] ] => *)
    (* rewrite is_true_split_or *)
   (* repeat (rewrite (@in_fsetU loc_ordType) ; rewrite Bool.orb_true_intro) ; try rewrite <- !fset1E ; try rewrite (ssrbool.introT (fset1P _ _) eq_refl) ; repeat (reflexivity || (left ; reflexivity) || right) *)
-  noramlize_fset ;
+  normalize_fset ;
   repeat (rewrite (@in_fsetU loc_ordType) ; rewrite (is_true_split_or_)) ; try rewrite <- !fset1E ; try rewrite (ssrbool.introT (fset1P _ _) eq_refl) ; repeat (reflexivity || (left ; reflexivity) || right)
   (* end *).
 
 Ltac solve_ssprove_obligations :=
   repeat (
-      intros ; noramlize_fset ;
+      intros ; autounfold ; normalize_fset ;
       (now solve_in_mem) (* TODO: add match goal *)
       || (now fset_equality) (* TODO: add match goal *)
       || (now solve_in_fset) (* TODO: add match goal *)
+      (* || (now solve_foldi_fsubset_trans) *)
       (* || (ssprove_valid_location || loc_incl_compute || opsig_incl_compute || ssprove_package_obligation) || *)
       (* (apply fsubsetxx || rewrite <- !fset0E ; apply fsub0set || now (try rewrite <- !fset0E ; try rewrite !fset0U ; try rewrite !fsetU0 ; try rewrite !fsetUA)) *)
       (* || (match goal with *)
@@ -2654,17 +2717,45 @@ Ltac solve_ssprove_obligations :=
       (* || now repeat rewrite <- fset_cat *)
       (* || (ssprove_valid_package ; ssprove_valid'_2) *)
       || (ssprove_valid'_2)
-      || ((try (Tactics.program_simpl; fail)))).
+      || ((now (* try *) (Tactics.program_simpl; fail)))).
+
+Ltac solve_fsubset_trans :=
+  now (solve_match || (refine (fsubset_trans _ _) ; [ | eassumption ] ; solve_ssprove_obligations)).
+
+Ltac solve_foldi_fsubset_trans :=
+  normalize_fset ;
+  repeat (rewrite is_true_split_and || rewrite fsubUset) ;
+  repeat (try rewrite andb_true_intro ; split) ;
+  repeat (solve_fsubset_trans || apply fsubsetU ; rewrite is_true_split_or ; ((left ; solve_fsubset_trans) || right)).
+  (* rewrite <- (ssrbool.elimT fsetUidPr i0). *)
+
+
+(* Equations foldi_both *)
+(*         {acc: choice_type} *)
+(*         {L1 L2 L3 I1 I2 I3} *)
+(*         (lo_hi: both L2 I2 uint_size * both L3 I3 uint_size) *)
+(*         (f: forall {L I} `{fsubset_loc : is_true (fsubset (L1 :|: (L2 :|: L3)) L)} `{fsubset_opsig : is_true (fsubset (I1 :|: (I2 :|: I3)) I)}, both (L2 :|: L3) (I2 :|: I3) uint_size -> both L I acc -> both ((L1 :|: (L2 :|: L3))) ((I1 :|: (I2 :|: I3))) (acc)) (* {i < hi} *) *)
+(*         (init: both L1 I1 acc) *)
+(*   : both (L1 :|: (L2 :|: L3)) (I1 :|: (I2 :|: I3)) (acc) := *)
+(*   foldi_both lo_hi f init := *)
+(*     solve_lift (@foldi acc (L1 :|: (L2 :|: L3)) L2 L3 (I1 :|: (I2 :|: I3)) I2 I3 (fst lo_hi) (snd lo_hi) (fun L I H0 H1 x y => solve_lift @f L I H0 H1 x y)) (solve_lift init). *)
+(* Solve All Obligations with intros ; (now solve_foldi_fsubset_trans || solve_ssprove_obligations). *)
 
 Equations foldi_both
         {acc: choice_type}
         {L1 L2 L3 I1 I2 I3}
         (lo_hi: both L2 I2 uint_size * both L3 I3 uint_size)
-        (f: forall {L I} `{fsubset_loc : is_true (fsubset L1 L)} `{fsubset_opsig : is_true (fsubset I1 I)}, both (L2 :|: L3) (I2 :|: I3) uint_size -> both L I acc -> both (L :|: (L2 :|: L3)) (I :|: (I2 :|: I3)) (acc)) (* {i < hi} *)
+        {L I}
+        (f: both (L2 :|: L3) (I2 :|: I3) uint_size ->
+            both L I acc ->
+            both L I acc)
         (init: both L1 I1 acc)
-         : both (L1 :|: (L2 :|: L3)) (I1 :|: (I2 :|: I3)) (acc) :=
+        `{is_true (fsubset (L1 :|: L2 :|: L3) L)} `{is_true (fsubset (I1 :|: I2 :|: I3) I)}
+         : both L I (acc) :=
   foldi_both lo_hi f init :=
-    foldi (fst lo_hi) (snd lo_hi) (@f) init.
+    foldi (fst lo_hi) (snd lo_hi) (@f) (init).
+Solve All Obligations with intros ; solve_ssprove_obligations ; solve_fsubset_trans.
+Fail Next Obligation.
 
 Notation "'fold'" :=
   (fun lo_hi init f => foldi_both (L1 := _) (L2 := _) (L3 := _) (I1 := _) (I2 := _) (I3 := _) lo_hi f init).
@@ -2702,20 +2793,36 @@ Fail Next Obligation.
 Notation "'ifb' b 'then' et 'else' ee" :=
   (if_both b et ee) (at level 100).
 
-Program Definition match_both {L1 L2 L3 I1 I2 I3} {A B} (x : both L3 I3 (option A)) (fa : both L3 I3 A -> both L1 I1 B) (fb : both L2 I2 B) `{fsubset_loc1 : is_true (fsubset L3 L1)}  `{fsubset_loc2 : is_true (fsubset L3 L2)}  `{fsubset_opsig1 : is_true (fsubset I3 I1)}  `{fsubset_opsig2 : is_true (fsubset I3 I2)} : both (L1 :|: L2) (I1 :|: I2) B :=
-  bind_both (fsubset_loc := _) (fsubset_opsig := _) x (fun y => match y with
-         | Some a => lift_both  (fsubset_loc := _) (fsubset_opsig := _) (fa (solve_lift (ret_both a)))
-         | None => lift_both  (fsubset_loc := _) (fsubset_opsig := _) fb
+Equations match_both_option {L1 L2 L3 I1 I2 I3} {A B} (x : both L3 I3 (option A)) (fa : both L3 I3 A -> both L1 I1 B) (fb : both L2 I2 B) `{fsubset_loc1 : is_true (fsubset L3 L1)}  `{fsubset_loc2 : is_true (fsubset L3 L2)}  `{fsubset_opsig1 : is_true (fsubset I3 I1)}  `{fsubset_opsig2 : is_true (fsubset I3 I2)} : both (L1 :|: L2) (I1 :|: I2) B :=
+  match_both_option x fa fb :=
+  bind_both x (fun y => match y with
+                     | Some a => solve_lift (fa (solve_lift (ret_both a)))
+                     | None => solve_lift fb
                      end).
 Solve All Obligations with solve_ssprove_obligations.
 Fail Next Obligation.
 
+Equations match_both_result {L1 L2 L3 I1 I2 I3} {A C B} (x : both L3 I3 (result C A)) (fa : both L3 I3 A -> both L1 I1 B) (fb : both L3 I3 C -> both L2 I2 B) `{fsubset_loc1 : is_true (fsubset L3 L1)}  `{fsubset_loc2 : is_true (fsubset L3 L2)}  `{fsubset_opsig1 : is_true (fsubset I3 I1)}  `{fsubset_opsig2 : is_true (fsubset I3 I2)} : both (L1 :|: L2) (I1 :|: I2) B :=
+  match_both_result x fa fb :=
+  bind_both x (fun y => match y with
+         | inl a => solve_lift (fa (solve_lift (ret_both a)))
+         | inr b => solve_lift (fb (solve_lift (ret_both b)))
+                                                             end).
+Solve All Obligations with
+  solve_ssprove_obligations.
+Fail Next Obligation.
+
 Notation "'matchb' x 'with' '|' 'Option_Some' a '=>' va '|' 'Option_None' '=>' vb 'end'" :=
-  (match_both x (fun a => va) vb (fsubset_loc1 := _) (fsubset_loc2 := _) (fsubset_opsig1 := _) (fsubset_opsig2 := _)).
+  (match_both_option x (fun a => va) vb (fsubset_loc1 := _) (fsubset_loc2 := _) (fsubset_opsig1 := _) (fsubset_opsig2 := _)).
 
 Notation "'matchb' x 'with' '|' 'Option_Some' a '=>' va '|' '_' '=>' vb 'end'" :=
-  (match_both x (fun a => va) vb (fsubset_loc1 := _) (fsubset_loc2 := _) (fsubset_opsig1 := _) (fsubset_opsig2 := _)).
+  (match_both_option x (fun a => va) vb (fsubset_loc1 := _) (fsubset_loc2 := _) (fsubset_opsig1 := _) (fsubset_opsig2 := _)).
 
+Notation "'matchb' x 'with' '|' 'Result_Ok' a '=>' va '|' 'Result_Err' b '=>' vb 'end'" :=
+  (match_both_result x (fun a => va) (fun b => vb) (fsubset_loc1 := _) (fsubset_loc2 := _) (fsubset_opsig1 := _) (fsubset_opsig2 := _)).
+
+Notation "'matchb' x 'with' '|' 'Result_Ok' a '=>' va '|' '_' '=>' vb 'end'" :=
+  (match_both_result x (fun a => va) (fun _ => vb) (fsubset_loc1 := _) (fsubset_loc2 := _) (fsubset_opsig1 := _) (fsubset_opsig2 := _)).
 
 Program Definition foldi_both0_
         {acc : choice_type}
@@ -2759,7 +2866,7 @@ Equations foldi_both0_list
         (f: both ((fset [])) ((fset [])) B -> both(fset []) (fset []) acc -> both (fset []) (fset []) (acc)) (* {i < hi} *)
         (init: both (fset []) (fset []) acc)
   : both (fset []) (fset []) (acc) :=
-  foldi_both0_list l f init := 
+  foldi_both0_list l f init :=
     bind_both l (fun l' => List.fold_left (fun x y => solve_lift @f (solve_lift ret_both y) (x) : both (fset []) (fset []) _) l' (solve_lift init : both (fset []) (fset []) _)).
 Solve Obligations with intros ; (assumption || solve_in_fset).
 Fail Next Obligation.
@@ -2772,3 +2879,606 @@ Fail Next Obligation.
 
 Notation "'ifb0' b 'then' et 'else' ee" :=
   (if_both0 b et ee) (at level 100).
+
+(* Definition Exception t  := (@choice_typeMonad.result_monad t). *)
+
+Notation "'letm[' bind_code_mnd ']' x ':=' y 'in' z" := (choice_typeMonad.monad_bind_both (BindCode := bind_code_mnd) y (fun x => z)) (at level 100, x pattern).
+Notation "'letm[' bind_code_mnd ']' ( x : t ) ':=' y 'in' z" := (choice_typeMonad.monad_bind_both (BindCode := bind_code_mnd) y (fun x => z)) (at level 100, x pattern).
+
+Check letm[ @choice_typeMonad.result_bind_code ('bool) ] y := solve_lift ret_both (choice_typeMonad.ret _) in _.
+
+(*** Hacspec-v2 specific fixes *)
+
+(* From Hacspec Require Import Hacspec_Lib. *)
+
+(* From Coq Require Import ZArith. *)
+(* Import List.ListNotations. *)
+(* Open Scope Z_scope. *)
+(* Open Scope bool_scope. *)
+
+(* Require Import Lia. *)
+(* Require Import Coq.Logic.FunctionalExtensionality. *)
+(* Require Import Sumbool. *)
+
+(* From mathcomp Require Import fintype. *)
+
+(* From Crypt Require Import choice_type Package Prelude. *)
+(* Import PackageNotation. *)
+(* From extructures Require Import ord fset fmap. *)
+
+(* From mathcomp Require Import ssrZ word. *)
+(* From Jasmin Require Import word. *)
+
+(* From Coq Require Import ZArith List. *)
+(* Import ListNotations. *)
+
+(* From Hacspec Require Import ChoiceEquality. *)
+(* From Hacspec Require Import LocationUtility. *)
+(* From Hacspec Require Import Hacspec_Lib_Comparable. *)
+(* From Hacspec Require Import Hacspec_Lib_Pre. *)
+(* From Hacspec Require Import Hacspec_Lib. *)
+
+(* Declare Scope hacspec_scope. *)
+
+(* Open Scope list_scope. *)
+(* Open Scope hacspec_scope. *)
+(* Open Scope nat_scope. *)
+
+(* Require Import Hacspec_Lib_Comparable. *)
+
+Import choice.Choice.Exports.
+Obligation Tactic := (* try timeout 8 *) solve_ssprove_obligations.
+
+(** Should be moved to Hacspec_Lib.v **)
+Program Definition int_xI {WS : wsize} (a : (* both (fset []) ([interface])  *)(@int WS)) : (* both (fset []) ([interface]) *) (@int WS) :=
+  Hacspec_Lib_Pre.int_add (Hacspec_Lib_Pre.int_mul a ((* lift_to_both (fset []) ([interface]) *) (@repr WS 2))) ((* lift_to_both (fset []) ([interface]) *) (@one WS)).
+(* Next Obligation. intros ; now do 2 rewrite fsetU0. Defined. *)
+(* Next Obligation. intros ; rewrite <- fset0E ; now do 2 rewrite fsetU0. Defined. *)
+
+Program Definition int_xO {WS : wsize} (a : int WS) : int WS :=
+  Hacspec_Lib_Pre.int_mul a (@repr WS 2).
+(* Next Obligation. intros ; now rewrite fsetU0. Defined. *)
+(* Next Obligation. intros ; rewrite <- fset0E ; now rewrite fsetU0. Defined. *)
+
+Definition both_int_one {WS : wsize} : both (fset []) ([interface]) (@int WS) := ret_both (one).
+
+Open Scope hacspec_scope.
+Definition int_num {WS : wsize} := int WS.
+Number Notation int_num Pos.of_num_int Pos.to_num_int (via positive mapping [[int_xI] => xI, [int_xO] => xO , [one] => xH]) : hacspec_scope.
+
+Notation "0" := (repr _ 0%Z) : hacspec_scope.
+
+(* Notation U8_t := int8. *)
+(* Notation U8 := id. *)
+(* Notation U16_t := int16. *)
+(* Notation U16 := id. *)
+(* Notation U32_t := int32. *)
+(* Notation U32 := id. *)
+(* Notation U64_t := int64. *)
+(* Notation U64 := id. *)
+(* Notation U128_t := int128. *)
+(* Notation U128 := id. *)
+
+Class Addition L1 L2 (* L3 *) I1 I2 (* I3 *) (A : choice_type) (* `(H_loc_fsubset13 : is_true (fsubset L1 L3)) `(H_opsig_fsubset13 : is_true (fsubset I1 I3)) `(H_loc_fsubset23 : is_true (fsubset L2 L3)) `(H_opsig_fsubset23 : is_true (fsubset I2 I3)) *) :=
+  add : both L1 I1 A -> both L2 I2 A -> both (L1 :|: L2) (* L3 *) (I1 :|: I2) (* I3 *) A.
+Notation "a .+ b" := (add a b).
+(* Instance array_add_inst {ws : wsize} {len: uint_size} {L1 L2 I1 I2} : Addition L1 L2 I1 I2 (nseq (int ws) len) := { add a b := a array_add b }. *)
+Instance int_add_inst {ws : wsize} {L1 L2 (* L3 *) I1 I2 (* I3 *)}  (* `{H_loc_fsubset13 : is_true (fsubset L1 L3)} `{H_opsig_fsubset13 : is_true (fsubset I1 I3)} `{H_loc_fsubset23 : is_true (fsubset L2 L3)} `{H_opsig_fsubset23 : is_true (fsubset I2 I3)} *) : Addition L1 L2 (* L3 *) I1 I2 (* I3 *) (@int ws) (* H_loc_fsubset13 H_opsig_fsubset13 H_loc_fsubset23 H_opsig_fsubset23 *) := { add a b := int_add (* (H_loc_incl_x := H_loc_fsubset13) (H_opsig_incl_x := H_opsig_fsubset13) (H_loc_incl_y := H_loc_fsubset23) (H_opsig_incl_y := H_opsig_fsubset23) *) a b }.
+
+Class Subtraction  L1 L2 (* L3 *) I1 I2 (* I3 *) (A : choice_type) (* `(H_loc_fsubset13 : is_true (fsubset L1 L3)) `(H_opsig_fsubset13 : is_true (fsubset I1 I3)) `(H_loc_fsubset23 : is_true (fsubset L2 L3)) `(H_opsig_fsubset23 : is_true (fsubset I2 I3)) *) :=
+  sub : both L1 I1 A -> both L2 I2 A -> both (L1 :|: L2) (* L3 *) (I1 :|: I2) (* I3 *) A.
+Notation "a .- b" := (sub a b (Subtraction := _)).
+(* Instance array_sub_inst {ws : wsize} {len: uint_size} {L1 L2 I1 I2} : Subtraction L1 L2 I1 I2 (nseq (@int ws) len) := { sub a b := a array_minus b }. *)
+Instance int_sub_inst {ws : wsize} {L1 L2 (* L3 *) I1 I2 (* I3 *)}  (* `{H_loc_fsubset13 : is_true (fsubset L1 L3)} `{H_opsig_fsubset13 : is_true (fsubset I1 I3)} `{H_loc_fsubset23 : is_true (fsubset L2 L3)} `{H_opsig_fsubset23 : is_true (fsubset I2 I3)} *) : Subtraction L1 L2 (* L3 *) I1 I2 (* I3 *) (@int ws) (* H_loc_fsubset13 H_opsig_fsubset13 H_loc_fsubset23 H_opsig_fsubset23 *) := { sub a b := int_sub (* (H_loc_incl_x := H_loc_fsubset13) (H_opsig_incl_x := H_opsig_fsubset13) (H_loc_incl_y := H_loc_fsubset23) (H_opsig_incl_y := H_opsig_fsubset23) *) a b }.
+
+Class Multiplication (L1 L2 (* L3 *) : {fset Location}) (I1 I2 (* I3 *) : Interface) A (* `(H_loc_incl1 : is_true (fsubset L1 L3)) (H_opsig_incl1 : is_true (fsubset I1 I3)) (H_loc_incl2 : is_true (fsubset L2 L3)) (H_opsig_incl2 : is_true (fsubset I2 I3)) *) := mul : both L1 I1 A -> both L2 I2 A -> both (L1 :|: L2) (* L3 *) (I1 :|: I2) (* I3 *)  A.
+Notation "a .* b" := (mul a b).
+(* Instance array_mul_inst {ws : wsize} {len: uint_size} { L1 L2 I1 I2} : Multiplication L1 L2 I1 I2 (nseq (@int ws) len) := { mul a b := a array_mul b }. *)
+Program Instance int_mul_inst {ws : wsize} { L1 L2 (* L3 *) : {fset Location} } { I1 I2 (* I3 *) : Interface} (* `{H_loc_incl1 : is_true (fsubset L1 L3)} `{H_opsig_incl1 : is_true (fsubset I1 I3)} `{H_loc_incl2 : is_true (fsubset L2 L3)} `{H_opsig_incl2 : is_true (fsubset I2 I3)} *) : Multiplication L1 L2 (* L3 *) I1 I2 (* I3 *) (@int ws) (* H_loc_incl1 H_opsig_incl1 H_loc_incl2 H_opsig_incl2 *) := { mul a b := int_mul a b }.
+Fail Next Obligation.
+
+Class Xor (L1 L2 (* L3 *) : {fset Location}) (I1 I2 (* I3 *) : Interface) A (* `(H_loc_incl1 : is_true (fsubset L1 L3)) (H_opsig_incl1 : is_true (fsubset I1 I3)) (H_loc_incl2 : is_true (fsubset L2 L3)) (H_opsig_incl2 : is_true (fsubset I2 I3)) *) := xor : both L1 I1 A -> both L2 I2 A -> both (L1 :|: L2) (* L3 *) (I1 :|: I2) (* I3 *)  A.
+Notation "a .^ b" := (xor a b).
+
+(* Instance array_xor_inst {ws : wsize} {len: uint_size} {L1 L2 I1 I2} : Xor L1 L2 I1 I2 (nseq (@int ws) len) := { xor a b := a array_xor b }. *)
+Program Instance int_xor_inst {ws : wsize} {L1 L2 (* L3 *) I1 I2 (* I3 *)} (* `{H_loc_incl1 : is_true (fsubset L1 L3)} `{H_opsig_incl1 : is_true (fsubset I1 I3)} `{H_loc_incl2 : is_true (fsubset L2 L3)} `{H_opsig_incl2 : is_true (fsubset I2 I3)} *) : Xor L1 L2 (* L3 *) I1 I2 (* I3 *) (@int ws) (* H_loc_incl1 H_opsig_incl1 H_loc_incl2 H_opsig_incl2 *) := { xor a b := int_xor a b }.
+Fail Next Obligation.
+
+(* Definition new {A : choice_type} {len} : nseq A len := array_new_ default _. *)
+
+(* (* Axiom conv : A -> B. *) *)
+(* (* Coercion conv : A >-> B. *) *)
+(* (* Check (fun x : A => x : B). *) *)
+
+(* Record mixin_of A := *)
+(*   Mixin { *)
+(*       as_nseq :> both A ; *)
+(*       as_seq :> both A ; *)
+(*     }. *)
+(* (* Check choice_type_class_of. *) *)
+(* Record class_of (A : choice_type) := { *)
+(*     base : choice.Choice.sort A ; *)
+(*     mixin : mixin_of A *)
+(*   }. *)
+(* Structure type := Pack {sort : choice_type ; _ : class_of sort }. *)
+
+(* Coercion mixin : class_of >-> mixin_of. *)
+(* Coercion sort : type >-> choice_type. *)
+
+Structure array_or_seq A L I (len : nat) :=
+  { as_nseq :> both L I (nseq_ A len) ;
+    as_seq :> both L I (seq A) ;
+    as_list :> both L I (chList A)
+  }.
+Print as_seq.
+Print as_nseq.
+
+Print Graph.
+
+(* Check (fun x : array_or_seq 'nat 25 => x : (* both_seq *) seq 'nat). *)
+(* Check (fun x : array_or_seq 'nat 25 => x : (* both_nseq *) (nseq 'nat 25)). *)
+
+Arguments as_seq {_} {_} {_} {_}. (* array_or_seq. *)
+Arguments as_nseq {_} {_} {_} {_}. (* array_or_seq. *)
+Arguments as_list {_} {_} {_} {_}. (* array_or_seq. *)
+(* Coercion as_seq : array_or_seq >-> both. *)
+(* Coercion as_nseq : array_or_seq >-> both. *)
+
+
+
+(* Check (fun x : array_or_seq 'nat fset0 (fset []) 25 => x : both (fset []) ([interface]) (nseq 'nat 25)). *)
+
+(* Definition nseq_array_or_seq {A L I len} (a : both L I (nseq A len)) := *)
+(*   Build_array_or_seq A L I len (array_to_seq a) a. *)
+(* Canonical (* Structure *) nseq_array_or_seq. *)
+
+Definition array_to_list {L I A n} := lift1_both (L := L) (I := I) (fun x => (@array_to_list A n x) : chList _).
+
+Definition seq_to_list {L I A} := lift1_both (L := L) (I := I) (fun x => (@seq_to_list A x) : chList _).
+
+Definition seq_from_list {L I A} := lift1_both (L := L) (I := I) (fun (x : chList _) => seq_from_list A (x : list _)).
+
+Definition array_from_list' {L I A} {n : nat} := lift1_both (L := L) (I := I) (fun (x : chList A) => @array_from_list' A x n : nseq_ _ _).
+
+Equations nseq_array_or_seq {A L I len} (val : both L I (nseq_ A len)) : array_or_seq A L I len :=
+  nseq_array_or_seq val := {| as_seq := array_to_seq val ; as_nseq := val ; as_list := array_to_list val |}.
+Fail Next Obligation.
+
+Arguments nseq_array_or_seq {A} {L} {I} {len}.
+Check nseq_array_or_seq.
+Coercion nseq_array_or_seq : both >-> array_or_seq.
+Canonical Structure nseq_array_or_seq.
+
+(* Check (fun (x : both (fset []) ([interface]) (nseq 'nat 25)) => x : array_or_seq 'nat fset0 (fset []) 25). *)
+
+(* (* TODO: use of is pure here is an issue!! *) *)
+(* Definition seq_array_or_seq {A : choice_type} {L I} (a : both L I (seq A)) : array_or_seq A L I (is_pure (seq_len (* (H_loc_incl_x := fsubsetxx _) (H_opsig_incl_x := fsubsetxx _) *) a : both L I _)) := *)
+(*   {| as_seq := a ; as_nseq := array_from_seq _ a ; |}. *)
+
+(* Coercion seq_array_or_seq : both >-> array_or_seq. *)
+(* Canonical Structure seq_array_or_seq. *)
+
+(* Definition seq_array_or_seq {A L I len} (a : both L I (seq A)) := *)
+(*   Build_array_or_seq A L I len a (array_from_seq (from_uint_size len) a). *)
+(* Canonical (* Structure *) seq_array_or_seq. *)
+(* Print Canonical Projections . *)
+
+(* Program Definition (* Equations *) array_index {A: choice_type} {len : nat} {L1 L2 I1 I2} (s: array_or_seq A L1 I1 len) {WS} (i : both L2 I2 (@int WS)) : both (L1 :|: L2) (I1 :|: I2) A := *)
+(*   (* array_index s i :=  *)Hacspec_Lib.array_index (as_nseq s) i. *)
+(* Fail Next Obligation. *)
+
+(* Definition array_index {A: choice_type} {len : uint_size} {L I} (s: both L I (nseq A len)) {WS} (i : both L I (@int WS)) := array_index s i. *)
+
+(* Definition size : forall {L I A len} {B} (H : {B = nseq A len} + {(B = seq A)}) (x : both L I B) `{len : match H with left _ => True | right b => len = eq_rect_r (fun B0 : choice_type => both L I B0 -> uint_size) (fun x' => is_pure (seq_len x')) b x end}, uint_size. *)
+(* Proof. *)
+(*   intros. *)
+(*   destruct H ; subst. *)
+(*   refine len. *)
+(*   refine (is_pure (seq_len x)). *)
+(*   Show Proof. *)
+(*   Show Proof. *)
+(* Qed.   *)
+
+(* Close Scope hacspec_scope. *)
+(* Print Prelude.positive. *)
+(* Definition len_of_nseq (H : choice_type) `{contra : match H with *)
+(*                            | chUnit => True *)
+(*                            | chMap (chFin (mkpos (S n) cond_pos) ) (A) => True *)
+(*                            | _ => False *)
+(*                                                     end} : nat. *)
+(*   refine *)
+(*   (match H as K return match K with *)
+(*                            | chUnit => True *)
+(*                            | chMap (chFin (mkpos (S n) cond_pos)) (A) => True *)
+(*                            | _ => False *)
+(*                                         end -> nat with *)
+(*    | chUnit => fun _ => 0%nat *)
+(*    | chMap (chFin (mkpos pos cond_pos)) A => *)
+(*        match pos as n return *)
+(*              match n with *)
+(*              | O => False *)
+(*              | _ => True *)
+(*              end -> nat *)
+(*        with *)
+(*        | O => fun m_contra => False_rect nat m_contra *)
+(*        | S n => fun _ => S n *)
+(*        end *)
+(*    | _ => fun m_contra => False_rect nat m_contra *)
+(*    end contra). *)
+
+Definition n_seq_array_or_seq {L I A} {B} (x : both L I B)
+           `(contra : match B with
+                      | chUnit => True
+                      | chMap (chFin (@mkpos (S n) _)) (C) => C = A
+                      | chMap 'nat (C) => C = A
+                      | chList C => C = A
+                      | _ => False
+                      end) :
+  let len := (match B as K return
+                    match K with
+                    | chUnit => True
+                    | chMap (chFin (@mkpos (S n) _)) (C) => C = A
+                    | chMap 'nat (C) => C = A
+                    | chList C => C = A
+                    | _ => False
+                    end -> nat
+              with
+              | chUnit => fun _ => 0%nat
+              | chMap (chFin (@mkpos p _)) C =>
+                  fun m_contra =>
+                    match p as p_ return match p_ with
+                                         | O => False
+                                         | _ => C = A
+                                         end -> nat
+                          with
+                  | O => fun m_contra => False_rect nat m_contra
+                  | S n => fun _ => S n
+                  end m_contra
+              | chMap 'nat C =>
+                  fun m_contra => 3%nat
+              | chList C => fun m_contra => 4%nat
+              | _ => fun m_contra => False_rect nat m_contra
+              end contra) in
+  array_or_seq A L I len.
+Proof.
+  intros.
+  destruct B ; try contradiction contra.
+  - change 'unit with (nseq_ A len) in x.
+    exact {| as_seq := array_to_seq x ; as_nseq := x; as_list := array_to_list x |}.
+  - destruct B1 ; try contradiction contra ; simpl in *.
+    + subst.
+      change (chMap 'nat A) with (seq A) in x.
+      exact ({| as_seq := x ; as_nseq := array_from_seq _ x ; as_list := seq_to_list x |}).
+    + destruct n.
+      destruct pos.
+      * contradiction.
+      * subst.
+        replace (chMap (chFin _) A) with (nseq_ A len) in x.
+        2:{
+          simpl.
+          f_equal.
+          f_equal.
+          apply (ssrbool.elimT (positive_eqP _ _)).
+          unfold positive_eq.
+          apply eqtype.eq_refl.
+        }
+        exact {| as_seq := array_to_seq x ; as_nseq := x; as_list := array_to_list x |}.
+  - subst.
+    exact {| as_seq := seq_from_list x ; as_nseq := array_from_list' x ; as_list := x |}.
+Defined.
+
+Notation " x '.a[' a ']'" := (array_index (n_seq_array_or_seq x _) a) (at level 40).
+
+(* Program Definition (* Equations *) array_upd {A: choice_type} {len : uint_size} {L1 L2 L3 I1 I2 I3} (s: both L1 I1 (nseq A len)) {WS} (i: both L2 I2 (@int WS)) (new_v: both L3 I3 A) : both (L1 :|: L2 :|: L3) (I1 :|: I2 :|: I3) (nseq A len) := *)
+(*   (* array_upd s i new_v := *) Hacspec_Lib.array_upd s i new_v. *)
+Fail Next Obligation.
+Notation " x '.a[' i ']<-' a" := (array_upd x i a) (at level 40).
+
+Notation update_at := array_upd.
+
+(* Definition update {A : Type}  `{Default A} {len slen} (s : nseq A len) {WS} (start : @int WS) (start_a : array_or_seq A slen) : nseq A len := *)
+(* array_update (a := A) (len := len) s (unsigned start) (as_seq start_a). *)
+
+(* Definition to_le_U32s {A l} := array_to_le_uint32s (A := A) (l := l). *)
+(* Axiom to_le_bytes : forall {ws : wsize} {len}, nseq (@int ws) len -> seq int8. *)
+(* Definition from_seq {A : Type}  `{Default A} {len slen} (s : array_or_seq A slen) : nseq A len := array_from_seq _ (as_seq s). *)
+
+Notation t_Seq := seq.
+(* Notation len := (fun s => seq_len s : int32). *)
+
+(* Definition array_slice {a: Type} `{Default a} {len : nat} (input: nseq a len) {WS} (start: @int WS) (slice_len: @int WS) : seq a := slice (array_to_seq input) (unsigned start) (unsigned (start .+ slice_len)). *)
+(* Notation slice := array_slice. *)
+(* Definition seq_new {A: Type} `{Default A} {WS} (len: @int WS) : seq A := seq_new (unsigned len). *)
+(* Notation new := seq_new. *)
+Notation num_exact_chunks := seq_num_exact_chunks.
+Notation get_exact_chunk := seq_get_exact_chunk.
+(* Definition set_chunk {a: Type} `{Default a} {len} (s: seq a) {WS} (chunk_len: @int WS) (chunk_num: @int WS) (chunk: array_or_seq a len) : seq a := seq_set_chunk s (unsigned chunk_len) (unsigned chunk_num) (as_seq chunk). *)
+(* Definition set_exact_chunk {a} `{H : Default a} {len} s {WS} := @set_chunk a H len s WS. *)
+Notation get_remainder_chunk := seq_get_remainder_chunk.
+Notation "a <> b" := (negb (eqb a b)).
+
+Notation from_secret_literal := nat_mod_from_secret_literal.
+(* Definition pow2 {m} (x : @int wsize32) := nat_mod_pow2 m (unsigned x). *)
+(* Instance nat_mod_addition {n} : Addition (nat_mod n) := { add a b := a +% b }. *)
+(* Instance nat_mod_subtraction {n} : Subtraction (nat_mod n) := { sub a b := a -% b }. *)
+(* Instance nat_mod_multiplication {n} : Multiplication (nat_mod n) := { mul a b := a *% b }. *)
+(* Definition from_slice {a: Type} `{Default a} {len slen} (x : array_or_seq a slen) {WS} (start: @int WS) (slice_len: @int WS) := array_from_slice default len (as_seq x) (unsigned start) (unsigned slice_len). *)
+Notation zero := nat_mod_zero.
+Notation to_byte_seq_le := nat_mod_to_byte_seq_le.
+Notation U128_to_le_bytes := u128_to_le_bytes.
+Notation U64_to_le_bytes := u64_to_le_bytes.
+     Notation from_byte_seq_le := nat_mod_from_byte_seq_le.
+Definition from_literal {m} := nat_mod_from_literal m.
+Notation inv := nat_mod_inv.
+Notation update_start := array_update_start.
+Notation pow := nat_mod_pow_self.
+Notation bit := nat_mod_bit.
+
+(* Definition int_to_int {ws1 ws2} (i : @int ws1) : @int ws2 := repr (unsigned i). *)
+(* Coercion int_to_int : int >-> int. *)
+(* Notation push := seq_push. *)
+Notation Build_secret := secret.
+Notation "a -× b" :=
+(prod a b) (at level 80, right associativity) : hacspec_scope.
+Notation Result_t := result.
+Axiom TODO_name : Type.
+Notation ONE := nat_mod_one.
+Notation exp := nat_mod_exp.
+(* Notation nat_mod := GZnZ.znz. *)
+(* Instance nat_mod_znz_addition {n} : Addition (GZnZ.znz n) := { add a b := a +% b }. *)
+(* Instance nat_mod_znz_subtraction {n} : Subtraction (GZnZ.znz n) := { sub a b := a -% b }. *)
+(* Instance nat_mod_znz_multiplication {n} : Multiplication (GZnZ.znz n) := { mul a b := a *% b }. *)
+Notation TWO := nat_mod_two.
+Notation ne := (fun x y => negb (eqb x y)).
+Notation eq := (eqb).
+Notation rotate_right := (ror).
+Notation to_be_U32s := array_to_be_uint32s.
+Notation get_chunk := seq_get_chunk.
+Notation num_chunks := seq_num_chunks.
+Notation U64_to_be_bytes := uint64_to_be_bytes.
+Notation to_be_bytes := array_to_be_bytes.
+Notation U8_from_usize := uint8_from_usize.
+Notation concat := seq_concat.
+Notation declassify := id.
+Notation U128_from_be_bytes := uint128_from_be_bytes.
+Notation U128_to_be_bytes := uint128_to_be_bytes.
+Notation slice_range := array_slice_range.
+Notation truncate := seq_truncate.
+(* Axiom array_to_be_uint64s : forall {A l}, nseq A l -> seq uint64. *)
+Notation to_be_U64s := array_to_be_uint64s.
+Notation classify := id.
+Notation U64_from_U8 := uint64_from_uint8.
+(* Definition Build_Range_t (a b : nat) := (a,b). (* match (b - a)%nat with O => [] | S n => match b with | O => [] | S b' => Build_Range_t a b' ++ [b] end end. *) *)
+
+Definition Build_t_Range {WS L1 L2 I1 I2} {f_start : both L1 I1 (int WS)} {f_end : both L2 I2 (int WS)} := (f_start,f_end).
+Notation Build_Range  := Build_t_Range.
+
+Notation declassify_eq := eq.
+Notation String_t := String.string.
+
+Notation "'i8(' v ')'" := (ret_both (v : int8) : both (fset []) ([interface]) _).
+Notation "'i16(' v ')'" := (ret_both (v : int16) : both (fset []) ([interface]) _).
+Notation "'i32(' v ')'" := (ret_both (v : int32) : both (fset []) ([interface]) _).
+Notation "'i64(' v ')'" := (ret_both (v : int64) : both (fset []) ([interface]) _).
+Notation "'i128(' v ')'" := (ret_both (v : int128) : both (fset []) ([interface]) _).
+
+Notation into_iter := (fun x => x).
+
+Definition (* vec_ *)len {L I A ws} := lift1_both (L := L) (I := I)  (fun (x : chList A) => repr ws (List.length x)).
+
+Definition andb {L1 L2 I1 I2} (x : both L1 I1 'bool) (y : both L2 I2 'bool) : both (L1 :|: L2) (I1 :|: I2) 'bool := lift2_both (fun (x y : 'bool) => Datatypes.andb x y : 'bool) x y.
+Definition negb {L1 I1} (x : both L1 I1 'bool) : both (L1) (I1) 'bool := lift1_both (fun (x : 'bool) => Datatypes.negb x : 'bool) x.
+Notation "a <> b" := (negb (eqb a b)).
+Notation "'not'" := (negb).
+Notation "x ':of:' y" := (x : both _ _ y) (at level 100).
+Notation "x ':of0:' y" := (x : both (fset []) (fset []) y) (at level 100).
+
+Class t_Serialize (Self : choice_type).
+Class t_Deserial (Self : choice_type).
+Class t_Serial (Self : choice_type).
+Notation "'t_Eq'" := (EqDec).
+(** end of: Should be moved to Hacspec_Lib.v **)
+
+Definition t_Result A B := result B A.
+
+(** Should be part of core.V **)
+
+Class t_Sized (A : choice_type) := Sized : A -> A.
+Class t_TryFrom (A : choice_type) := TryFrom : A -> A.
+Class t_Into (A : choice_type) := Into : A -> A.
+Class t_PartialEq (A : choice_type) := PartialEq : A -> A.
+Class t_Copy (A : choice_type) := Copy : A -> A.
+Class t_Clone (A : choice_type) := Clone : A -> A.
+Definition t_Option : choice_type -> choice_type := chOption.
+Inductive vec_typ :=
+| t_Global.
+Definition t_Vec : choice_type -> vec_typ -> choice_type := fun A _ => chList A.
+
+Notation t_Default := Default.
+(* Class t_Default A := { default : A }. *)
+
+#[global] Instance bool_copy : t_Copy 'bool := {Copy x := x}.
+#[global] Instance bool_clone : t_Clone 'bool := {Clone x := x}.
+#[global] Instance bool_sized : t_Sized 'bool := {Sized x := x}.
+
+Definition ilog2 {WS} {L I} (x : both L I (int WS)) : both L I (int WS) := x. (* TODO *)
+
+Definition collect {A} {L I} (x : both L I (chList A)) : both L I (t_Vec A t_Global) := x.
+
+
+Equations swap_both_list {A L I} (x : list (both L I A)) : both L I (chList A) :=
+  swap_both_list x :=
+  (List.fold_left (fun (x : both L I (chList A)) y =>
+   bind_both x (fun x' =>
+   bind_both y (fun y' =>
+   solve_lift (ret_both ((y' :: x') : chList A))))) x (solve_lift (ret_both ([] : chList A)))).
+Solve All Obligations with solve_ssprove_obligations.
+Fail Next Obligation.
+
+Equations match_list {A B : choice_type} {L I} (x : both L I (chList A)) (f : list A -> B) : both L I B :=
+  match_list x f :=
+  bind_both x (fun x' => solve_lift (ret_both (f x'))).
+Solve All Obligations with solve_ssprove_obligations.
+Fail Next Obligation.
+
+Equations map {A B} {L I} (x : both L I (chList A))  (f : both L I A -> both L I B) : both L I (chList B) :=
+  map x f :=
+  bind_both x (fun x' => swap_both_list (List.map (fun y => f (solve_lift (ret_both y))) x')).
+Solve All Obligations with solve_ssprove_obligations.
+Fail Next Obligation.
+
+Definition cloned {A} {L I} (x : both L I (chList A)) : both L I (chList A) := x.
+
+Equations iter {A L I} (x : both L I (seq A)) : both L I (chList A) :=
+  iter x :=
+  bind_both x (fun x' => solve_lift (ret_both (Hacspec_Lib_Pre.seq_to_list _ x' : chList A))).
+Solve All Obligations with solve_ssprove_obligations.
+Fail Next Obligation.
+
+Definition dedup {A} {L I} (x : both L I (t_Vec A t_Global)) : both L I (t_Vec A t_Global) := x.
+
+Definition t_String := Coq.Strings.String.string.
+Equations new {A L I} : both L I (t_Vec A t_Global) :=
+  new := solve_lift (ret_both ([] : chList A)).
+Solve All Obligations with solve_ssprove_obligations.
+Fail Next Obligation.
+
+Definition enumerate {A} {L I} (x : both L I (t_Vec A t_Global)) : both L I (t_Vec A t_Global) := x.
+
+(* Inductive ControlFlow {L I} (A : choice_type) (B : choice_type) := *)
+(* | ControlFlow_Continue (val : both L I A) *)
+(* | ControlFlow_Break (val : both L I B). *)
+
+(* Definition run {A B : choice_type} {L I} (x : ControlFlow A B) : both L I (t_Result A B) := *)
+(*   match x with *)
+(*   | ControlFlow_Continue v => Ok v *)
+(*   | ControlFlow_Break v => Err v *)
+(*   end. *)
+
+(* Program Definition build_under_impl_1 {A B} : (t_Result A B) := *)
+(*   run (letb layers := (match branch (build_tree_under_impl_1 partial_layers depth) with *)
+(*     | ControlFlow_Break residual => letb hoist1 := (v_Break (from_residual residual)) : both _ _ (t_Never) in *)
+(*       ControlFlow_Continue (never_to_any hoist1) *)
+(*     | ControlFlow_Continue val => ControlFlow_Continue val *)
+(*     end) in *)
+(*   ControlFlow_Continue (Result_Ok (Build_PartialTree layers))). *)
+(* Fail Next Obligation. *)
+
+(*** More functions *)
+Definition t_Drain : choice_type -> vec_typ -> choice_type := t_Vec.
+Inductive t_Range := RangeFull.
+Equations drain : forall {L I A}, both L I (t_Vec A t_Global) -> t_Range -> both L I (t_Drain A t_Global × t_Vec A t_Global) :=
+  drain x _ :=
+    bind_both x (fun x' => solve_lift (ret_both ((x', []) : (t_Drain A t_Global × t_Vec A t_Global)))).
+Solve All Obligations with solve_ssprove_obligations.
+Fail Next Obligation.
+Notation t_Rev := id.
+Equations rev {L I A} (x : both L I (chList A)) : both L I (chList A) := rev x := bind_both x (fun x => solve_lift (ret_both (List.rev x : chList _))).
+Solve All Obligations with solve_ssprove_obligations.
+Fail Next Obligation.
+
+Definition pop {L I A} : both L I (chList A) -> both L I (chOption A × t_Vec A (t_Global)) :=
+  lift1_both (fun (x : chList A) => (List.hd_error x , List.tl x) : (chOption A × t_Vec A (t_Global))).
+
+Definition push {L1 L2 I1 I2 A} : both L1 I1 (t_Vec A t_Global) -> both L2 I2 A -> both (L1 :|: L2) (I1 :|: I2) (t_Vec A (t_Global)) :=
+  lift2_both (fun  (x : chList A) y => y :: x : chList A).
+
+Notation Option_Some := Some.
+Definition append {L1 L2 I1 I2} {A : choice_type} (l : both L1 I1 (chList A)) (x : both L2 I2 (chList A)) : both (L2 :|: L1) (I2 :|: I1) (chList A × chList A) :=
+  lift2_both (fun (x : chList A) (y : chList A) => (app y x, []) : chList A × chList A) x l.
+
+Notation clone := id.
+Definition seq_unzip {A B} (s : chList (A × B)) : chList A × chList B := (seq.unzip1 s, seq.unzip2 s).
+Definition unzip {L I} {A B} : both L I (chList (A × B)) -> both L I (chList A × chList B) := lift1_both seq_unzip.
+Equations deref {L I A} : both L I (t_Vec A t_Global) -> both L I (seq A) :=
+  deref X := bind_both X (fun x : t_Vec A t_Global => solve_lift (ret_both (Hacspec_Lib_Pre.seq_from_list A x))).
+Solve All Obligations with solve_ssprove_obligations.
+Fail Next Obligation.
+Definition t_Never := False.
+(* Notation v_Break := id. *)
+Notation Result_Err := Err.
+Notation Result_Ok := Ok.
+
+Notation "'ret_both' 'tt'" := (ret_both (tt : 'unit)).
+
+(** Should be part of concordium.v **)
+Class HasInitContext (Self : choice_type).
+Class t_HasInitContext (Self : choice_type) (something : choice_type).
+Class t_HasActions (Self : choice_type) := {accept : forall {L I}, both L I Self}.
+Class HasReceiveContext (Self : choice_type).
+Definition t_ParamType := 'unit.
+Definition t_ParseError := 'unit.
+(* (t_RegisterParam) *)
+Class t_HasReceiveContext (Self : choice_type) (something : choice_type) := { get : forall {Ctx L I}, both L I (t_ParamType × t_Result Ctx (t_ParseError)) }.
+Arguments get {Self} {something} (t_HasReceiveContext) {Ctx} {L} {I}.
+
+Definition parameter_cursor {T : _} `{ t_Sized (T)} `{ t_HasReceiveContext (T) ('unit)} `{ t_Sized (T)} `{ t_HasReceiveContext (T) ('unit)} {L1 : {fset Location}} {I1 : Interface} (ctx : both L1 I1 (T)) : t_HasReceiveContext (T) ('unit) := _.
+
+Notation "'matchb' 'branch' x 'with' '|' 'ControlFlow_Break' a '=>' va '|' 'ControlFlow_Continue' b '=>' vb 'end'" :=
+  (match_both_result x (fun b => vb) (fun a => va) (fsubset_loc1 := _) (fsubset_loc2 := _) (fsubset_opsig1 := _) (fsubset_opsig2 := _)).
+
+(* Section ExceptionMonad. *)
+(*   Definition exception (A R : choice_type) := (A -> R) -> R. *)
+(*   Definition exception_bind {A B R} (c : (exception A R)) (f : A -> (exception B R)) : (exception B R) := (fun k => (c (fun t => f t k))). *)
+(*   Definition exception_ret {A R : choice_type} (a : A) : (exception A R) := *)
+(*     fun f => f a. *)
+(*   (* Cannot be monad, as we are missing chArrow ! *) *)
+(* End ExceptionMonad. *)
+
+(* Program Definition run {L I} {A} {R : choice_type} `{Default R} (e : exception A (both L I R)) : (both L I R) := *)
+(*   e (fun _ => solve_lift (ret_both Hacspec_Lib_Comparable.default)). *)
+
+(* Definition exception (A R : Type) := (A -> R) -> R. *)
+(* Definition exception_bind {A B R} (c : (exception A R)) (f : A -> (exception B R)) : (exception B R) := (fun k => (c (fun t => f t k))). *)
+(* Definition exception_ret {A R : choice_type} (a : A) : (exception A R) := *)
+(*   fun f => f a. *)
+(* (* Cannot be monad, as we are missing chArrow ! *) *)
+(* (* Definition run {T T' R} : ((T -> exception T' R) -> exception T R) -> exception T R := fun f k => f (fun t x => k t) k. *) *)
+(* Program Definition run {L I} {R : choice_type} (e : exception (both L I R) (both L I R)) : (both L I R) := e id. *)
+
+(* Definition v_Break {L I A R} (v : both L I R) : exception A (both L I R) := (fun f => v). *)
+
+(* Notation "'lete' x ':=' y 'in' z" := (exception_bind y (fun x => z)) (at level 100, x pattern). *)
+(* Equations exception_test {L : {fset Location}} {I : Interface} : both L I (int8) := *)
+(*   exception_test  := *)
+(*     solve_lift (run (lete _ := v_Break (ret_both (1 : int8)) in *)
+(*                        ControlFlow_Continue (ret_both (0 : int8)))) : both L I (int8). *)
+(* Next Obligation. *)
+(*   apply nat. *)
+(* Qed. *)
+(* Fail Next Obligation. *)
+
+Notation ControlFlow_Continue := Result_Ok.
+Notation v_Break := Result_Err.
+Notation never_to_any := id.
+Notation "'matchb' 'branch' x 'with' '|' 'ControlFlow_Break' a '=>' va '|' 'ControlFlow_Continue' b '=>' vb 'end'" :=
+  (match_both_result x (fun b => vb) (fun a => va) (fsubset_loc1 := _) (fsubset_loc2 := _) (fsubset_opsig1 := _) (fsubset_opsig2 := _)).
+Equations run {L I A} (x : both L I (choice_typeMonad.M (CEMonad := (@choice_typeMonad.mnd (choice_typeMonad.result_bind_code A))) A)) : both L I A :=
+  run x :=
+  bind_both x (fun y => match y with
+                             | inl r | inr r => solve_lift ret_both r
+                             end).
+Fail Next Obligation.
+
+Notation from_residual := Result_Err.
+
+Ltac remove_duplicate_pair :=
+  normalize_fset ;
+  repeat match goal with
+  | |- context G [(?a :|: (?a :|: ?c))] =>
+      replace (a :|: (a :|: c)) with (a :|: a :|: c) by (now rewrite <- fsetUA) ; rewrite fsetUid
+  end.
+
+
+Axiom t_Reject : choice_type.
+Equations repeat {L1 L2 I1 I2} {A} (e : both L1 I1 A) (n : both L2 I2 uint_size) : both (L1 :|: L2) (I1 :|: I2) (nseq A (is_pure n)) :=
+  repeat e n :=
+ (eq_rect
+       (Datatypes.length (List.repeat (solve_lift e) (Z.to_nat (unsigned (is_pure n)))))
+       (fun n0 : nat => both (L1 :|: L2) (I1 :|: I2) (nseq_ A n0)) (bind_both e
+       (fun _ : A =>
+        array_from_list (List.repeat (solve_lift e) (Z.to_nat (unsigned (is_pure n)))))
+)
+       (Z.to_nat (unsigned (is_pure n)))
+       (List.repeat_length (solve_lift e) (Z.to_nat (unsigned (is_pure n))))).
+Fail Next Obligation.
